Strata/Languages/C_Simp/DDMTransform/Translate.lean
@@ -275,14 +275,15 @@ def translateMeasure (bindings : TransBindings) (arg : Arg) : TransM (Option (LE
                       return some (← translateExpr bindings e[0]!))
                   arg
 
-def translateInvariant (bindings : TransBindings) (arg : Arg) : TransM (List (LExpr CSimpLParams.mono)) := do
+def translateInvariant (bindings : TransBindings) (arg : Arg) :
+    TransM (List (String × LExpr CSimpLParams.mono)) := do
   translateOption (fun maybe_arg => do
                     match maybe_arg with
                     | none => return []
                     | some a =>
                       let e ← checkOpArg a q`C_Simp.invariant 1
                       assert! e.size == 1
-                      return [← translateExpr bindings e[0]!])
+                      return [("", ← translateExpr bindings e[0]!)])
                   arg
 
 ---------------------------------------------------------------------
